theorems.ml
@@ -219,6 +219,18 @@ let RIGHT_AND_DISTRIB = prove
 
 export_thm RIGHT_AND_DISTRIB;;
 
+let IMP_AND_DISTRIB = prove
+ (`!p q r. (p ==> q /\ r) <=> (p ==> q) /\ (p ==> r)`,
+  ITAUT_TAC);;
+
+export_thm IMP_AND_DISTRIB;;
+
+let OR_IMP_DISTRIB = prove
+ (`!p q r. (p \/ q ==> r) <=> (p ==> r) /\ (q ==> r)`,
+  ITAUT_TAC);;
+
+export_thm OR_IMP_DISTRIB;;
+
 (* ------------------------------------------------------------------------- *)
 (* Degenerate cases of quantifiers.                                          *)
 (* ------------------------------------------------------------------------- *)
